@@ -1,65 +1,25 @@
 module
 
 public import Roolean.QfBv.Bitvector
+public import Roolean.QfBv.Domain
 
-public inductive UniOperator
-  | Not
-  | Neg
+public inductive Primary (w: Nat) where
+  | Constant (constant: Bitvector w)
+  | Variable (index: USize)
 deriving Repr, Inhabited
 
-public inductive BiOperator
-  | Add
-  | Sub
-  | Mul
-  | Udiv
-  | Urem
-  | Sdiv
-  | Srem
-  | BitAnd
-  | BitOr
-  | BitXor
-  | Eq
-  | Ne
-  | Implies
-  | Ult
-  | Ule
-  | Ugt
-  | Uge
-  | Slt
-  | Sle
-  | Sgt
-  | Sge
-  | Shl
-  | Lshr
-  | Ashr
-deriving Repr, Inhabited
+public inductive Formula: Nat → Type where
+  | Leaf: {n: Nat} → Primary n → Formula n
+  | Unary: {n: Nat} → Formula n → UniOp → Formula n
+  | BinaryNormal: {n: Nat} → Formula n → Formula n → BiNormalOp → Formula n
+  | BinaryReduction: {n: Nat} → Formula n → Formula n → BiReductionOp → Formula 1
+deriving Repr, Nonempty
 
-mutual
 
-public inductive Formula where
+/-
   | Constant (w: Nat) (constant: Bitvector w)
   | Variable (index: USize)
-  | Operation (operation: Operation)
-deriving Repr, Inhabited
-
-public inductive BiOp where
-  | Mk (op: BiOperator) (left: Formula) (right: Formula)
-deriving Repr, Inhabited
-
-public inductive Operation where
-  | Unary (op: UniOperator) (inner: Formula)
-  | Binary (op: BiOperator) (left: Formula) (right: Formula)
-  -- TODO others
-/-  | Ext (ext: ExtOp)
-  | Ite (ite: IteOp)
-  | Concat (concat: ConcatOp)
-  | Extract (extract: ExtractOp)
-  | Rotate (rotate: RotateOp) -/
-deriving Repr, Inhabited
-
-end
-
-public structure Problem where
-  public variables: Array BitvectorType
-  public formula: Formula
-deriving Repr, Inhabited
+  | Unary (op: UniOperator) (inner: Formula w)
+  | Binary (op: BiOperator) (a: Nat) (left: Formula a) (right: Formula a)
+-/
+--deriving Repr, Inhabited
